code/k256/Hacl.Spec.K256.GLV.Lemmas.fst
@@ -502,125 +502,148 @@ let lemma_point_mul_double_split_lambda k1 p1 k2 p2 =
 
 //-----------------------------------
 
-// -[k]P = [k](-P)
-val aff_point_negate_cond_pow_lemma: p:S.aff_point -> k:nat ->
-  Lemma (LE.pow S.mk_k256_comm_monoid (S.aff_point_negate p) k ==
-    S.aff_point_negate (LE.pow S.mk_k256_comm_monoid p k))
+// // [k]P or -[k]P = [k](-P)
+// val aff_point_negate_cond_pow_lemma: is_negate:bool -> p:S.aff_point -> k:nat ->
+//   Lemma (aff_point_negate_cond (SE.pow SM.aff_mk_k256_concrete_ops p k) is_negate ==
+//     SE.pow SM.aff_mk_k256_concrete_ops (aff_point_negate_cond p is_negate) k)
 
-let aff_point_negate_cond_pow_lemma p k =
-  LE.lemma_inverse_pow S.mk_k256_abelian_group p k
+// let aff_point_negate_cond_pow_lemma is_negate p k =
+//   let co = SM.aff_mk_k256_concrete_ops in
+//   let cm = S.mk_k256_comm_monoid in
 
-
-// [k]P or -[k]P = [k](-P)
-val point_negate_cond_pow_lemma: is_negate:bool -> p:S.proj_point -> k:nat ->
-  Lemma (S.to_aff_point (SE.pow S.mk_k256_concrete_ops (point_negate_cond p is_negate) k) ==
-    S.to_aff_point (point_negate_cond (SE.pow S.mk_k256_concrete_ops p k) is_negate))
-
-let point_negate_cond_pow_lemma is_negate p k =
-  let p_aff = S.to_aff_point p in
-  let co = S.mk_k256_concrete_ops in
-  let cm = S.mk_k256_comm_monoid in
-
-  if is_negate then
-    calc (==) {
-      S.to_aff_point (SE.pow co (S.point_negate p) k);
-      (==) { SE.pow_lemma co (S.point_negate p) k }
-      LE.pow cm (S.to_aff_point (S.point_negate p)) k;
-      (==) { LS.to_aff_point_negate_lemma p }
-      LE.pow cm (S.aff_point_negate p_aff) k;
-      (==) { aff_point_negate_cond_pow_lemma p_aff k }
-      S.aff_point_negate (LE.pow cm p_aff k);
-      (==) { SE.pow_lemma co p k }
-      S.aff_point_negate (S.to_aff_point (SE.pow co p k));
-      (==) { LS.to_aff_point_negate_lemma (SE.pow co p k) }
-      S.to_aff_point (S.point_negate (SE.pow co p k));
-    }
+//   if is_negate then
+//     calc (==) {
+//       S.aff_point_negate (SE.pow co p k);
+//       (==) { SE.pow_lemma co p k }
+//       S.aff_point_negate (LE.pow cm p k);
+//       (==) { LE.lemma_inverse_pow S.mk_k256_abelian_group p k }
+//       LE.pow cm (S.aff_point_negate p) k;
+//       (==) { SE.pow_lemma co (S.aff_point_negate p) k }
+//       SE.pow co (S.aff_point_negate p) k;
+//     }
+//   else ()
 
 
-// [k](-[lambda]P) = [lambda](-[k]P)
-val aff_point_negate_cond_lambda_pow_lemma: p:S.aff_point -> k:nat ->
-  Lemma (LE.pow S.mk_k256_comm_monoid (S.aff_point_negate (aff_point_mul lambda p)) k ==
-    aff_point_mul lambda (S.aff_point_negate (LE.pow S.mk_k256_comm_monoid p k)))
+//--------------------------
 
-let aff_point_negate_cond_lambda_pow_lemma p k =
-  let ag = S.mk_k256_abelian_group in
-  let cm = S.mk_k256_comm_monoid in
-  let p_k = LE.pow cm p k in
-  let p_lambda = S.aff_point_mul lambda p in
+// // -[k]P = [k](-P)
+// val aff_point_negate_cond_pow_lemma: p:S.aff_point -> k:nat ->
+//   Lemma (LE.pow S.mk_k256_comm_monoid (S.aff_point_negate p) k ==
+//     S.aff_point_negate (LE.pow S.mk_k256_comm_monoid p k))
 
-  calc (==) {
-    LE.pow cm (S.aff_point_negate p_lambda) k;
-    (==) { LE.lemma_inverse_pow ag p_lambda k }
-    S.aff_point_negate (LE.pow cm p_lambda k);
-    (==) { LE.lemma_pow_mul cm p lambda k }
-    S.aff_point_negate (LE.pow cm p (lambda * k));
-    (==) { LE.lemma_pow_mul cm p k lambda }
-    S.aff_point_negate (LE.pow cm p_k lambda);
-    (==) { LE.lemma_inverse_pow ag p_k lambda }
-    aff_point_mul lambda (S.aff_point_negate p_k);
-  }
+// let aff_point_negate_cond_pow_lemma p k =
+//   LE.lemma_inverse_pow S.mk_k256_abelian_group p k
 
 
-// [k]([lambda]P) = [lambda]([k]P)
-val aff_point_cond_lambda_pow_lemma: p:S.aff_point -> k:nat ->
-  Lemma (LE.pow S.mk_k256_comm_monoid (aff_point_mul lambda p) k ==
-    aff_point_mul lambda (LE.pow S.mk_k256_comm_monoid p k))
+// // [k]P or -[k]P = [k](-P)
+// val point_negate_cond_pow_lemma: is_negate:bool -> p:S.proj_point -> k:nat ->
+//   Lemma (S.to_aff_point (SE.pow S.mk_k256_concrete_ops (point_negate_cond p is_negate) k) ==
+//     S.to_aff_point (point_negate_cond (SE.pow S.mk_k256_concrete_ops p k) is_negate))
 
-let aff_point_cond_lambda_pow_lemma p k =
-  let cm = S.mk_k256_comm_monoid in
-  calc (==) {
-    LE.pow cm (LE.pow cm p lambda) k;
-    (==) { LE.lemma_pow_mul cm p lambda k }
-    LE.pow cm p (lambda * k);
-    (==) { LE.lemma_pow_mul cm p k lambda }
-    LE.pow cm (LE.pow cm p k) lambda;
-  }
+// let point_negate_cond_pow_lemma is_negate p k =
+//   let p_aff = S.to_aff_point p in
+//   let co = S.mk_k256_concrete_ops in
+//   let cm = S.mk_k256_comm_monoid in
+
+//   if is_negate then
+//     calc (==) {
+//       S.to_aff_point (SE.pow co (S.point_negate p) k);
+//       (==) { SE.pow_lemma co (S.point_negate p) k }
+//       LE.pow cm (S.to_aff_point (S.point_negate p)) k;
+//       (==) { LS.to_aff_point_negate_lemma p }
+//       LE.pow cm (S.aff_point_negate p_aff) k;
+//       (==) { aff_point_negate_cond_pow_lemma p_aff k }
+//       S.aff_point_negate (LE.pow cm p_aff k);
+//       (==) { SE.pow_lemma co p k }
+//       S.aff_point_negate (S.to_aff_point (SE.pow co p k));
+//       (==) { LS.to_aff_point_negate_lemma (SE.pow co p k) }
+//       S.to_aff_point (S.point_negate (SE.pow co p k));
+//     }
+
+// // [k](-[lambda]P) = [lambda](-[k]P)
+// val aff_point_negate_cond_lambda_pow_lemma: p:S.aff_point -> k:nat ->
+//   Lemma (LE.pow S.mk_k256_comm_monoid (S.aff_point_negate (aff_point_mul lambda p)) k ==
+//     aff_point_mul lambda (S.aff_point_negate (LE.pow S.mk_k256_comm_monoid p k)))
+
+// let aff_point_negate_cond_lambda_pow_lemma p k =
+//   let ag = S.mk_k256_abelian_group in
+//   let cm = S.mk_k256_comm_monoid in
+//   let p_k = LE.pow cm p k in
+//   let p_lambda = S.aff_point_mul lambda p in
+
+//   calc (==) {
+//     LE.pow cm (S.aff_point_negate p_lambda) k;
+//     (==) { LE.lemma_inverse_pow ag p_lambda k }
+//     S.aff_point_negate (LE.pow cm p_lambda k);
+//     (==) { LE.lemma_pow_mul cm p lambda k }
+//     S.aff_point_negate (LE.pow cm p (lambda * k));
+//     (==) { LE.lemma_pow_mul cm p k lambda }
+//     S.aff_point_negate (LE.pow cm p_k lambda);
+//     (==) { LE.lemma_inverse_pow ag p_k lambda }
+//     aff_point_mul lambda (S.aff_point_negate p_k);
+//   }
 
 
-// [k]([lambda]P) = [lambda]([k]P) or [k](-[lambda]P) = [lambda](-[k]P)
-val point_negate_cond_lambda_pow_lemma: is_negate:bool -> p:S.proj_point -> k:nat ->
-  Lemma (let co = S.mk_k256_concrete_ops in
-    S.to_aff_point (SE.pow co (point_negate_cond (point_mul_lambda p) is_negate) k) ==
-    S.to_aff_point (point_mul_lambda (point_negate_cond (SE.pow co p k) is_negate)))
+// // [k]([lambda]P) = [lambda]([k]P)
+// val aff_point_cond_lambda_pow_lemma: p:S.aff_point -> k:nat ->
+//   Lemma (LE.pow S.mk_k256_comm_monoid (aff_point_mul lambda p) k ==
+//     aff_point_mul lambda (LE.pow S.mk_k256_comm_monoid p k))
 
-let point_negate_cond_lambda_pow_lemma is_negate p k =
-  let co = S.mk_k256_concrete_ops in
-  let cm = S.mk_k256_comm_monoid in
-  let p_aff = S.to_aff_point p in
-  let p_k = SE.pow co p k in
-  let p_k_neg = S.point_negate (SE.pow co p k) in
-  let p_lambda = point_mul_lambda p in
-  let p_lambda_neg = S.point_negate p_lambda in
+// let aff_point_cond_lambda_pow_lemma p k =
+//   let cm = S.mk_k256_comm_monoid in
+//   calc (==) {
+//     LE.pow cm (LE.pow cm p lambda) k;
+//     (==) { LE.lemma_pow_mul cm p lambda k }
+//     LE.pow cm p (lambda * k);
+//     (==) { LE.lemma_pow_mul cm p k lambda }
+//     LE.pow cm (LE.pow cm p k) lambda;
+//   }
 
-  if is_negate then
-    calc (==) {
-      S.to_aff_point (SE.pow co p_lambda_neg k);
-      (==) { SE.pow_lemma co p_lambda_neg k }
-      LE.pow cm (S.to_aff_point p_lambda_neg) k;
-      (==) { LS.to_aff_point_negate_lemma p_lambda }
-      LE.pow cm (S.aff_point_negate (S.to_aff_point p_lambda)) k;
-      (==) { lemma_glv p }
-      LE.pow cm (S.aff_point_negate (S.aff_point_mul lambda p_aff)) k;
-      (==) { aff_point_negate_cond_lambda_pow_lemma p_aff k }
-      aff_point_mul lambda (S.aff_point_negate (LE.pow cm p_aff k));
-      (==) { SE.pow_lemma co p k }
-      aff_point_mul lambda (S.aff_point_negate (S.to_aff_point (SE.pow co p k)));
-      (==) { LS.to_aff_point_negate_lemma (SE.pow co p k) }
-      aff_point_mul lambda (S.to_aff_point p_k_neg);
-      (==) { lemma_glv p_k_neg }
-      S.to_aff_point (point_mul_lambda p_k_neg);
-    }
-  else
-    calc (==) {
-      S.to_aff_point (SE.pow co (point_mul_lambda p) k);
-      (==) { SE.pow_lemma co (point_mul_lambda p) k }
-      LE.pow cm (S.to_aff_point (point_mul_lambda p)) k;
-      (==) { lemma_glv p }
-      LE.pow cm (LE.pow cm p_aff lambda) k;
-      (==) { aff_point_cond_lambda_pow_lemma p_aff k }
-      LE.pow cm (LE.pow cm p_aff k) lambda;
-      (==) { SE.pow_lemma co p k }
-      LE.pow cm (S.to_aff_point p_k) lambda;
-      (==) { lemma_glv p_k }
-      S.to_aff_point (point_mul_lambda p_k);
-    }
+
+// // [k]([lambda]P) = [lambda]([k]P) or [k](-[lambda]P) = [lambda](-[k]P)
+// val point_negate_cond_lambda_pow_lemma: is_negate:bool -> p:S.proj_point -> k:nat ->
+//   Lemma (let co = S.mk_k256_concrete_ops in
+//     S.to_aff_point (SE.pow co (point_negate_cond (point_mul_lambda p) is_negate) k) ==
+//     S.to_aff_point (point_mul_lambda (point_negate_cond (SE.pow co p k) is_negate)))
+
+// let point_negate_cond_lambda_pow_lemma is_negate p k =
+//   let co = S.mk_k256_concrete_ops in
+//   let cm = S.mk_k256_comm_monoid in
+//   let p_aff = S.to_aff_point p in
+//   let p_k = SE.pow co p k in
+//   let p_k_neg = S.point_negate (SE.pow co p k) in
+//   let p_lambda = point_mul_lambda p in
+//   let p_lambda_neg = S.point_negate p_lambda in
+
+//   if is_negate then
+//     calc (==) {
+//       S.to_aff_point (SE.pow co p_lambda_neg k);
+//       (==) { SE.pow_lemma co p_lambda_neg k }
+//       LE.pow cm (S.to_aff_point p_lambda_neg) k;
+//       (==) { LS.to_aff_point_negate_lemma p_lambda }
+//       LE.pow cm (S.aff_point_negate (S.to_aff_point p_lambda)) k;
+//       (==) { lemma_glv p }
+//       LE.pow cm (S.aff_point_negate (S.aff_point_mul lambda p_aff)) k;
+//       (==) { aff_point_negate_cond_lambda_pow_lemma p_aff k }
+//       aff_point_mul lambda (S.aff_point_negate (LE.pow cm p_aff k));
+//       (==) { SE.pow_lemma co p k }
+//       aff_point_mul lambda (S.aff_point_negate (S.to_aff_point (SE.pow co p k)));
+//       (==) { LS.to_aff_point_negate_lemma (SE.pow co p k) }
+//       aff_point_mul lambda (S.to_aff_point p_k_neg);
+//       (==) { lemma_glv p_k_neg }
+//       S.to_aff_point (point_mul_lambda p_k_neg);
+//     }
+//   else
+//     calc (==) {
+//       S.to_aff_point (SE.pow co (point_mul_lambda p) k);
+//       (==) { SE.pow_lemma co (point_mul_lambda p) k }
+//       LE.pow cm (S.to_aff_point (point_mul_lambda p)) k;
+//       (==) { lemma_glv p }
+//       LE.pow cm (LE.pow cm p_aff lambda) k;
+//       (==) { aff_point_cond_lambda_pow_lemma p_aff k }
+//       LE.pow cm (LE.pow cm p_aff k) lambda;
+//       (==) { SE.pow_lemma co p k }
+//       LE.pow cm (S.to_aff_point p_k) lambda;
+//       (==) { lemma_glv p_k }
+//       S.to_aff_point (point_mul_lambda p_k);
+//     }
